example related to option type

compiler_test/beepl_test/BeePL_external_call.v
@@ -1,4 +1,4 @@
-Require Import Integers AST Ctypes BeePL BeeTypes BeePL_values. 
+Require Import Integers AST Ctypes BeePL BeeTypes BeePL_values BeePL_notations BeePL_typechecker. 
 From Coq Require Import String ZArith.
 From compcert Require Import Csyntaxdefs.
 Import Csyntaxdefs.CsyntaxNotations.
@@ -32,67 +32,73 @@ Definition ident_to_string : list (ident * string) := ((_a, "a") ::
                                                       (_main, "main") :: nil).
 
 Definition prim_expr : BeePL.expr := Prim (Ref) 
-                                          (Var _b (Ptype (BeeTypes.Tint I32 Signed dattr)) :: nil)
-                                          (Reftype _b (Bprim (Tint Ctypes.I32 Ctypes.Signed dattr)) dattr).
+                                          (Var _b tint32s :: nil) trint32s.
 
-Definition test : BeePL.expr := (App (Var _add (Ftype (Ptype (BeeTypes.Tint I32 Signed dattr) ::
-                                                       Reftype _b (Bprim (Tint Ctypes.I32 Ctypes.Signed dattr)) dattr :: nil) (* args type signature *)
+Definition test : BeePL.expr := (App (Var _add (tfun (tint32s :: trint32s :: nil)(* args type signature *)
                                                       (nil) (* effect *)
-                                                      (Ptype (BeeTypes.Tint I32 Signed dattr)))) (* return type *)
-                                     (Var _a (Ptype (BeeTypes.Tint I32 Signed dattr)) :: 
+                                                      tint32s)) (* return type *)
+                                     (Var _a tint32s :: 
                                       Prim (Ref) 
-                                           (Var _b (Ptype (BeeTypes.Tint I32 Signed dattr)) :: nil)
-                                           (Reftype _b (Bprim (Tint Ctypes.I32 Ctypes.Signed dattr)) dattr) :: nil)
-                                     (Ptype (BeeTypes.Tint I32 Signed dattr))).
+                                           (Var _b tint32s :: nil) trint32s :: nil) tint32s).
 
 Definition f_external_call : BeePL.function := {| 
-                                   fn_return := (Ptype (BeeTypes.Tint I32 Signed dattr));
-                                   fn_effect := nil;
+                                   fn_return := tint32s;
+                                   fn_effect := (Alloc mem_ident :: nil);
                                    fn_callconv := cc_default;
                                    fn_args := nil;
-                                   fn_vars := ((_a, BeeTypes.Ptype (BeeTypes.Tint Ctypes.I32 Ctypes.Signed dattr)) :: 
-                                               (_b, BeeTypes.Ptype (BeeTypes.Tint Ctypes.I32 Ctypes.Signed dattr)) :: 
-                                               (_c, BeeTypes.Ptype (BeeTypes.Tint Ctypes.I32 Ctypes.Signed dattr)) :: nil);
+                                   fn_vars := ((_a, tint32s) :: 
+                                               (_b, tint32s) :: 
+                                               (_c, tint32s) :: nil);
                                    fn_body := Bind 
-                                                (_a) 
-                                                (Ptype (BeeTypes.Tint I32 Signed dattr))
-                                                (Const (ConsInt (Int.repr 1)) (Ptype (BeeTypes.Tint I32 Signed dattr)))
+                                                (_a) tint32s
+                                                (cint (Int.repr 1) tint32s) 
                                                 (Bind 
-                                                   (_b) 
-                                                   (Ptype (BeeTypes.Tint I32 Signed dattr))
-                                                   (Const (ConsInt (Int.repr 2)) (Ptype (BeeTypes.Tint I32 Signed dattr)))
+                                                   (_b) tint32s
+                                                   (cint (Int.repr 2) tint32s) 
                                                    (Bind 
-                                                      (_c) 
-                                                      (Ptype (BeeTypes.Tint I32 Signed dattr))
-                                                      (App (Var _add (Ftype (Ptype (BeeTypes.Tint I32 Signed dattr) ::
-                                                                             Reftype _b (Bprim (Tint Ctypes.I32 Ctypes.Signed dattr)) dattr :: nil) (* args type signature *)
+                                                      (_c) tint32s 
+                                                      (App (Var _add (Ftype (tint32s :: trint32s :: nil) (* args type signature *)
                                                                             (nil) (* effect *)
-                                                                            (Ptype (BeeTypes.Tint I32 Signed dattr)))) (* return type *)
-                                                           (Var _a (Ptype (BeeTypes.Tint I32 Signed dattr)) :: 
+                                                                            tint32s)) (* return type *)
+                                                           (Var _a tint32s :: 
                                                             Prim (Ref) 
-                                                                 (Var _b (Ptype (BeeTypes.Tint I32 Signed dattr)) :: nil)
-                                                                 (Reftype _b (Bprim (Tint Ctypes.I32 Ctypes.Signed dattr)) dattr) :: nil)
-                                                           (Ptype (BeeTypes.Tint I32 Signed dattr)))
-                                                      (Var _c (Ptype (BeeTypes.Tint I32 Signed dattr)))
-                                                      (Ptype (BeeTypes.Tint I32 Signed dattr)))
-                                                   (Ptype (BeeTypes.Tint I32 Signed dattr)))
-                                                (Ptype (BeeTypes.Tint I32 Signed dattr)) |}.
+                                                                 (Var _b tint32s :: nil) trint32s :: nil) tint32s)
+                                                      (Var _c tint32s) tint32s) tint32s) tint32s |}.
+
 
 Definition add_external_function : BeePL.external_function
    := EF_external "add" 
-      {| bsig_args := (Ptype (BeeTypes.Tint I32 Signed dattr) :: 
-                       Reftype _a (Bprim (Tint Ctypes.I32 Ctypes.Signed dattr)) dattr :: nil);
+      {| bsig_args := tint32s :: trint32s :: nil;
          bsig_ef := nil;
-         bsig_res := Ptype (BeeTypes.Tint I32 Signed dattr);
+         bsig_res := tint32s;
          bsig_cc := cc_default
       |}.
 
 Definition global_definitions : list (ident * AST.globdef BeePL.fundef type) 
-   := (_add, AST.Gfun(BeePL.External (add_external_function)
-                                     (Ptype (BeeTypes.Tint I32 Signed dattr) :: 
-                                      Reftype _a (Bprim (Tint Ctypes.I32 Ctypes.Signed dattr)) dattr :: nil)
-                                     (Ptype (BeeTypes.Tint I32 Signed dattr))
+   := (_add, AST.Gfun(BeePL.External (add_external_function) (tint32s :: trint32s :: nil) tint32s 
                                      (cc_default))) :: 
       (_main, AST.Gfun(BeePL.Internal (f_external_call))):: nil.
 
-Definition public_idents : list ident := (_main :: nil).
+Definition public_idents : list ident := (_main :: _add :: nil).
+
+Definition bcomposites : list bcomposite_definition := nil.
+
+Lemma bcomposite_correct :
+  wf_bcomposites bcomposites.
+Proof.
+  unfold wf_bcomposites.
+  unfold build_bcomposite_env; simpl; reflexivity.
+Qed.
+
+Definition example1 : BeePL.program := @mkbprogram bcomposites 
+                                                   global_definitions 
+                                                   public_idents 
+                                                   _main 
+                                                   bcomposite_correct
+                                                   ident_to_string.
+
+
+(*Compute (type_check_expr example1.(prog_comp_env) 
+                         (bind_vars (bind_vars empty_context f_external_call.(fn_args)) f_external_call.(fn_vars)) empty_context f_external_call.(fn_body)).
+
+Compute (type_check_program example1).*) (* Type checks *)
