compiler_test/beepl_test/BeePL_match_fail_ex1.v
@@ -1,20 +1,18 @@
 Require Import Integers AST Ctypes BeePL BeeTypes BeePL_values BeePL_typechecker. 
 From Coq Require Import String ZArith Lists.List.
-From compcert Require Import Csyntaxdefs Errors Maps BeePL_aux BeePL_Option_Struct.
+From compcert Require Import Csyntaxdefs Errors Maps BeePL_aux BeePL_notations.
 Import Csyntaxdefs.CsyntaxNotations.
 Local Open Scope string_scope.
 Local Open Scope csyntax_scope.
 
-(* This program should not be allowed by the compiler as we only allow option containing pointers *)
 (* int main() {
    option<int> r;
-   r = Some 4;
    y = match r with
         | None => 0
-        | Some x => x
+        | Some x => !r
    return y; }
 *)
-
+(*
 Definition dattr := {| attr_volatile := false; attr_alignas := None |}.
 Definition _r : ident := $"r".
 Definition _x : ident := $"x".
@@ -29,28 +27,21 @@ Definition ident_to_string : list (ident * string) := ((_r, "r") ::
                                                        (_main, "main") :: nil).
 
 Definition f_option1 : BeePL.function := {| 
-                                   fn_return := (Ptype (BeeTypes.Tint I32 Unsigned dattr));
-                                   fn_effect := nil;
+                                   fn_return := tint32s;
+                                   fn_effect := Write mem_ident :: Read mem_ident :: nil;
                                    fn_callconv := cc_default;
                                    fn_args := nil;
-                                   fn_vars := ((_r, BeeTypes.Otype (Ptype (BeeTypes.Tint Ctypes.I32 Ctypes.Unsigned dattr))) :: 
-                                               (_x, (Ptype (BeeTypes.Tint Ctypes.I32 Ctypes.Unsigned dattr))) ::
-                                               (_y, (Ptype (BeeTypes.Tint Ctypes.I32 Ctypes.Unsigned dattr))) :: 
-                                               (_t, (Ptype (BeeTypes.Tint Ctypes.I32 Ctypes.Unsigned dattr))) :: nil);
-                                   fn_body := Bind _t (Ptype Tunit)
-                                                 (Prim Massgn ((Var _r (BeeTypes.Otype (Ptype (BeeTypes.Tint Ctypes.I32 Ctypes.Unsigned dattr)))) :: 
-                                                               (Esome (Const (ConsInt (Int.repr 4)) (Ptype (BeeTypes.Tint I32 Unsigned dattr)))
-                                                                   (BeeTypes.Otype (Ptype (BeeTypes.Tint Ctypes.I32 Ctypes.Unsigned dattr)))) :: nil) 
-                                                 (Ptype Tunit))
-                                               (Bind _y (Ptype (BeeTypes.Tint Ctypes.I32 Ctypes.Unsigned dattr)) 
-                                                     (Match (Var _r (BeeTypes.Otype (Ptype (BeeTypes.Tint Ctypes.I32 Ctypes.Unsigned dattr))))
+                                   fn_vars := ((_r, toption tint32s) :: 
+                                               (_x, tint32s) ::
+                                               (_y, tint32s) :: 
+                                               (_t, tint32s) :: nil);
+                                   fn_body := Bind _r (toption tint32s)
+                                               (Bind _y tint32s 
+                                                     (Match (Var _r (toption tint32s))
                                                               (Pnone :: Psome _x :: nil) 
-                                                              (Const (ConsInt (Int.repr 0)) (Ptype (BeeTypes.Tint I32 Unsigned dattr)) ::
-                                                               Var _x (Ptype (BeeTypes.Tint I32 Unsigned dattr)) :: nil) 
-                                                             (Ptype (BeeTypes.Tint I32 Unsigned dattr)))
-                                                     (Var _y (Ptype (BeeTypes.Tint Ctypes.I32 Ctypes.Unsigned dattr)))
-                                                (Ptype (BeeTypes.Tint Ctypes.I32 Ctypes.Unsigned dattr)))
-                                               (Ptype (BeeTypes.Tint Ctypes.I32 Ctypes.Unsigned dattr))|}.
+                                                              (cint (Int.repr 0) tint32s ::
+                                                               Prim Deref (Var _r (toption tint32s) :: nil) tint32s :: nil) tint32s) 
+                                                     (Var _y tint32s) tint32s) tint32s |}.
 
 
 Definition global_definitions : list (ident * AST.globdef BeePL.fundef type) 
@@ -66,6 +57,15 @@ Lemma bcomposite_correct :
 Proof.
   unfold wf_bcomposites.
   unfold build_bcomposite_env; simpl; reflexivity.
-Qed.
+Qed.*)
 
-(*Compute (get_bcs_from_globdefs (unzip2 global_definitions)).*)
+(*Definition example1 : BeePL.program := @mkbprogram bcomposites 
+                                                   global_definitions 
+                                                   public_idents 
+                                                   _main 
+                                                   bcomposite_correct
+                                                   ident_to_string.*)
+
+(*Compute (type_check_expr example1.(prog_comp_env) 
+                         (bind_vars (bind_vars empty_context f_option1.(fn_args)) f_option1.(fn_vars)) empty_context f_option1.(fn_body)).
+Compute (type_check_program example1). *) (* Type checks *)
