compiler_test/beepl_test/BeePL_progs.v
@@ -3,7 +3,12 @@ Require Import BeePL BeeTypes Errors BeePL_typechecker Csyntaxdefs.
 From Coq Require Import String.
 
 Require Import BeePL_add BeePL_add_ptr BeePL_div_zero1 BeePL_div_zero BeePL_add_ex1
-BeePL_cond BeePL_app BeePL_funptr_ex1. (* BeePL_app  BeePL_external_call BeePL_ref.
+BeePL_cond BeePL_app BeePL_funptr_ex1 BeePL_bpf_get_prandom BeePL_for_ex1 BeePL_for_ex2
+BeePL_external_call BeePL_match_fail_ex1 BeePL_null_ptr. 
+
+
+
+(* BeePL_app  BeePL_external_call BeePL_ref.
 Require Import BeePL_struct_ex2 BeePL_for_ex1 BeePL_for_ex2 BeePL_globvar1.
 Require Import BeePL_bpf_get_prandom BeePL_bpf_ktime_get_ns.*) (*BeePL_null_ptr BeePL_match_fail_ex1.*)
 
@@ -24,11 +29,11 @@ Require Import BeePL_bpf_get_prandom BeePL_bpf_ktime_get_ns.*) (*BeePL_null_ptr 
 
 (* Construct the BeePL.program *)
 
-Definition example1 : BeePL.program := @mkbprogram BeePL_funptr_ex1.bcomposites 
-                                                   BeePL_funptr_ex1.global_definitions 
-                                                   BeePL_funptr_ex1.public_idents 
-                                                   BeePL_funptr_ex1._main 
-                                                   BeePL_funptr_ex1.bcomposite_correct
-                                                   BeePL_funptr_ex1.ident_to_string.
+Definition example1 : BeePL.program := @mkbprogram BeePL_null_ptr.bcomposites 
+                                                   BeePL_null_ptr.global_definitions 
+                                                   BeePL_null_ptr.public_idents 
+                                                   BeePL_null_ptr._main 
+                                                   BeePL_null_ptr.bcomposite_correct
+                                                   BeePL_null_ptr.ident_to_string.
 
 
